/inti/unprivil/AllPassed

AbstractPlatform/IntegrityProof.bpl
@@ -1,9 +1,55 @@
 function uf_load_data(i_eid : tap_enclave_id_t, vaddr : vaddr_t, iter : int) : word_t;
 
+// The computation performed by the enclave. (non-inline)
+procedure EnclaveFetchComputation(iter : int) 
+    returns (ret_op : word_t)
+
+    modifies cpu_mem;
+    modifies cpu_regs;
+    modifies cpu_pc;
+    modifies cache_valid_map, cache_tag_map, cpu_addr_valid;
+
+    requires tap_enclave_metadata_valid[cpu_enclave_id];
+    requires tap_addr_perm_x(cpu_addr_valid[cpu_pc]);
+    requires cpu_owner_map[cpu_addr_map[cpu_pc]] == cpu_enclave_id;
+
+    // cut branches
+    // requires !tap_enclave_metadata_privileged[eid];
+    // description / ensures
+{
+    var r0, r1  : word_t;
+    var rd      : regindex_t;
+    var eid     : tap_enclave_id_t; // current (protected) Enclave's eid
+    var i_eid   : tap_enclave_id_t; // PE's inspection id 
+    var pc_pa   : wap_addr_t;
+    var pc_op   : word_t;
+    var l_vaddr : vaddr_t;
+    var l_data  : word_t;
+    var s_vaddr : vaddr_t;
+    var s_data  : word_t;
+    var excp    : exception_t;
+    var hit     : bool;
+    var way     : cache_way_index_t;
+
+    eid := cpu_enclave_id;
+    pc_pa := cpu_addr_map[cpu_pc];
+    assert tap_enclave_metadata_addr_excl[eid][cpu_pc];
+    assert tap_addr_perm_x(cpu_addr_valid[cpu_pc]);
+
+    //  cut branches
+    assert !tap_enclave_metadata_privileged[eid];
+
+    havoc way; assume valid_cache_way_index(way);
+    call pc_op, excp, hit := fetch_va(cpu_pc, way);
+    assert excp == excp_none;
+
+    ret_op := pc_op;
+}
+
 // The computation performed by the enclave.
 procedure {:inline 1} EnclaveComputation(iter : int)
-    // returns (vaddr : vaddr_t, paddr : wap_addr_t, data : word_t)
-    returns (ret_r0 : word_t, ret_r1 : word_t)
+    returns (vaddr : vaddr_t, paddr : wap_addr_t, data : word_t)
+    // returns (ret_op : word_t)
 
     modifies cpu_mem;
     modifies cpu_regs;
@@ -28,7 +74,6 @@ procedure {:inline 1} EnclaveComputation(iter : int)
     var hit     : bool;
     var way     : cache_way_index_t;
 
-
     // debug assignments
     // vaddr := k0_vaddr_t;
     // paddr := k0_wap_addr_t;
@@ -47,61 +92,63 @@ procedure {:inline 1} EnclaveComputation(iter : int)
     call pc_op, excp, hit := fetch_va(cpu_pc, way);
     assert excp == excp_none;
 
+    // ret_op := pc_op;
     // two register sources.
+    // ret_rindex := uf_cpu_r0_index(pc_op);
     r0 := cpu_regs[uf_cpu_r0_index(pc_op)];
     r1 := cpu_regs[uf_cpu_r1_index(pc_op)];
 
-    ret_r0 := r0;
-    ret_r1 := r1;
+    // ret_r0 := r0;
+    // ret_r1 := r1;
 
     // load address and value.
-    // l_vaddr := uf_mem_load_vaddr(cpu_pc, pc_op, r0, r1);
-    // assume tap_addr_perm_r(cpu_addr_valid[l_vaddr]);
+    l_vaddr := uf_mem_load_vaddr(cpu_pc, pc_op, r0, r1);
+    assume tap_addr_perm_r(cpu_addr_valid[l_vaddr]);
 
-    // // select load target && ensure load validity
-    // i_eid := uf_mem_load_eid(cpu_pc, pc_op, r0, r1);
-    // if (tap_enclave_metadata_privileged[eid]) {
-    //     assume tap_enclave_metadata_owner_map[i_eid] == eid; 
-    // } else {
-    //     assume i_eid == eid;
-    // }
+    // select load target && ensure load validity
+    i_eid := uf_mem_load_eid(cpu_pc, pc_op, r0, r1);
+    if (tap_enclave_metadata_privileged[eid]) {
+        assume tap_enclave_metadata_owner_map[i_eid] == eid; 
+    } else {
+        assume i_eid == eid;
+    }
     
-    // // data from NE can also be cached (PIPT)
-    // // data from outside cannot be cached
-    // if (tap_enclave_metadata_addr_excl[i_eid][l_vaddr]) {
-    //     assert cpu_owner_map[tap_enclave_metadata_addr_map[i_eid][l_vaddr]] == i_eid;
-    //     havoc way; assume valid_cache_way_index(way);
-    //     call l_data, excp, hit := load_va(i_eid, l_vaddr, way);
-    //     assert excp == excp_none;
-    // } else {
-    //     hit := false;
-    //     excp := excp_none;
-    //     l_data := uf_load_data(i_eid, l_vaddr, iter);
-    // }
+    // data from NE can also be cached (PIPT)
+    // data from outside cannot be cached
+    if (tap_enclave_metadata_addr_excl[i_eid][l_vaddr]) {
+        assert cpu_owner_map[tap_enclave_metadata_addr_map[i_eid][l_vaddr]] == i_eid;
+        havoc way; assume valid_cache_way_index(way);
+        call l_data, excp, hit := load_va(i_eid, l_vaddr, way);
+        assert excp == excp_none;
+    } else {
+        hit := false;
+        excp := excp_none;
+        l_data := uf_load_data(i_eid, l_vaddr, iter);
+    }
 
-    // // get data to store to mem.
-    // s_vaddr := uf_mem_store_vaddr(cpu_pc, pc_op, l_data, r0, r1);
-    // s_data := uf_mem_store_data(cpu_pc, pc_op, l_data, r0, r1);
-    // vaddr := s_vaddr;
-    // paddr := cpu_addr_map[s_vaddr];
-    // data := s_data;
-    // // update mem.
-    // assume tap_addr_perm_w(cpu_addr_valid[s_vaddr]);
-    // if (tap_enclave_metadata_addr_excl[eid][s_vaddr]) {
-    //     assert (cpu_owner_map[cpu_addr_map[s_vaddr]] == eid);
-    //     havoc way; assume valid_cache_way_index(way);
-    //     call excp, hit := store_va(s_vaddr, s_data, way);
-    //     assert excp == excp_none;
-    // }
+    // get data to store to mem.
+    s_vaddr := uf_mem_store_vaddr(cpu_pc, pc_op, l_data, r0, r1);
+    s_data := uf_mem_store_data(cpu_pc, pc_op, l_data, r0, r1);
+    vaddr := s_vaddr;
+    paddr := cpu_addr_map[s_vaddr];
+    data := s_data;
+    // update mem.
+    assume tap_addr_perm_w(cpu_addr_valid[s_vaddr]);
+    if (tap_enclave_metadata_addr_excl[eid][s_vaddr]) {
+        assert (cpu_owner_map[cpu_addr_map[s_vaddr]] == eid);
+        havoc way; assume valid_cache_way_index(way);
+        call excp, hit := store_va(s_vaddr, s_data, way);
+        assert excp == excp_none;
+    }
 
-    // // update pc.
-    // cpu_pc := uf_cpu_pc(cpu_pc, pc_op, l_data, r0, r1);
-    // assume tap_addr_perm_x(cpu_addr_valid[cpu_pc]);
-    // assume tap_enclave_metadata_addr_excl[eid][cpu_pc];
-    // assert cpu_owner_map[cpu_addr_map[cpu_pc]] == eid;
-    // // update regs.
-    // rd := uf_cpu_r2_index(pc_op);
-    // cpu_regs[rd] := uf_cpu_result(cpu_pc, pc_op, l_data, r0, r1);
+    // update pc.
+    cpu_pc := uf_cpu_pc(cpu_pc, pc_op, l_data, r0, r1);
+    assume tap_addr_perm_x(cpu_addr_valid[cpu_pc]);
+    assume tap_enclave_metadata_addr_excl[eid][cpu_pc];
+    assert cpu_owner_map[cpu_addr_map[cpu_pc]] == eid;
+    // update regs.
+    rd := uf_cpu_r2_index(pc_op);
+    cpu_regs[rd] := uf_cpu_result(cpu_pc, pc_op, l_data, r0, r1);
 }
 
 procedure {:inline 1} IntegrityAdversarialStep(
@@ -236,8 +283,7 @@ procedure {:inline 1} IntegrityEnclaveStep(
     /* what operation?  */  op : tap_proof_op_t, 
     /* which iteration? */  iter : int
 )
-    returns (next_mode : mode_t, vaddr : vaddr_t, paddr : wap_addr_t, data : word_t,
-             r0 : word_t, r1 : word_t)
+    returns (next_mode : mode_t, vaddr : vaddr_t, paddr : wap_addr_t, data : word_t)
 
     modifies cpu_mem;
     modifies cpu_regs;
@@ -280,10 +326,11 @@ procedure {:inline 1} IntegrityEnclaveStep(
     var way               : cache_way_index_t;
 
     // debug 
+    // retop := k0_word_t;
     // lvaddr := k0_vaddr_t;
-    r0 := k0_word_t;
-    r1 := k0_word_t;    
-
+    // r0 := k0_word_t;
+    // r1 := k0_word_t;    
+    // rindex := 513;  // default value: exceed 
     // debug end
     
     eid   := cpu_enclave_id;
@@ -307,7 +354,7 @@ procedure {:inline 1} IntegrityEnclaveStep(
         next_mode := mode_untrusted;
     } else if (op == tap_proof_op_compute) {
         // call vaddr, paddr, data, lvaddr := EnclaveComputation(iter);
-        call r0, r1 := EnclaveComputation(iter);
+        call vaddr, paddr, data := EnclaveComputation(iter);
         next_mode := mode_enclave;      
     }
 
@@ -461,8 +508,9 @@ procedure ProveIntegrity()
 
     // debug variables
     var pc_op_1, pc_op_2    : word_t;
-    var lvaddr_1, lvaddr_2  : vaddr_t;
-    var r0_1, r0_2, r1_1, r1_2 : word_t;
+    // var lvaddr_1, lvaddr_2  : vaddr_t;
+    // var r0_1, r0_2, r1_1, r1_2 : word_t;
+    // var rindex_1, rindex_2 : regindex_t;
     // cut branches: 
     //  launch PE
     assume !e_privileged;
@@ -698,18 +746,18 @@ procedure ProveIntegrity()
 
             // enclave step in trace_1
             call RestoreContext_1();
-            call current_mode, vaddr_1, paddr_1, data_1, r0_1, r1_1 := IntegrityEnclaveStep(
+            call current_mode, vaddr_1, paddr_1, data_1 := IntegrityEnclaveStep(
                                                             e_proof_op, iter);
             call SaveContext_1();
 
             // enclave step in trace_2
             call RestoreContext_2();
-            call current_mode, vaddr_2, paddr_2, data_2, r0_2, r1_2 := IntegrityEnclaveStep(
+            call current_mode, vaddr_2, paddr_2, data_2 := IntegrityEnclaveStep(
                                                             e_proof_op, iter);
             call SaveContext_2();
 
-            assert r0_1 == r0_2;
-            assert r1_1 == r1_2;
+            // assert pc_op_1 == pc_op_2;
+            // assert rindex_1 == rindex_2;
             assert vaddr_1 == vaddr_2;
             assert data_1 == data_2;
         }
